Finish "record" functions
- And they got moved back to the programming language itself. Seems I
  couldn't abstract it into a separate file. Perhaps if I use 'Include'
  to include the source code, it would work...

He4/Discussion/NatRangeIterator.v
@@ -54,6 +54,8 @@ Inductive tm : Type :=
   | tnewex : clex -> tm
   | tclex : clex -> tm -> tm.
 
+Definition tempty := tvoid.
+
 Inductive value : tm -> Prop :=
 
   (* Base types *)
@@ -64,11 +66,153 @@ Inductive value : tm -> Prop :=
   | vpair : forall t1 t2, value t1 -> value t2 -> value (tpair t1 t2)
   | vclex : forall clex t1, value t1 -> value (tclex clex t1).
 
-Definition stack := @ProgramState.stack (prod ty tm).
-Definition store := @ProgramState.store (prod ty tm).
-Definition sk_read (n : nat) (sk : stack) := ProgramState.sk_read n sk (pair Tvoid tvoid).
-Definition sr_read (n : nat) (sr : store) := ProgramState.sr_read n sr (pair Tvoid tvoid).
-Definition sf_new (n : nat) := ProgramState.repeat (pair Tvoid tvoid) n.
+Section Stacks.
+Definition stack := ProgramState.stack tm.
+Definition sk_read_hd (n : nat) (sk : stack) : tm := ProgramState.sk_read_hd n sk tempty.
+Definition sk_resize_hd (n : nat) (sk : stack) : stack := ProgramState.sk_resize_hd n sk tempty.
+End Stacks.
+
+Section Stores.
+Definition store := ProgramState.store tm.
+Definition sr_read (n : nat) (sr : store) : tm := ProgramState.sr_read n sr tempty.
+End Stores.
+
+Section Records.
+
+(** Records encoded as nested pair terms. *)
+
+Hint Resolve Lt.lt_S_n.
+
+Inductive is_rc : tm -> Prop :=
+  | RC_tempty : is_rc tempty
+  | RC_tpair : forall t rc, is_rc rc -> is_rc (tpair t rc).
+
+Fixpoint rc_create (n : nat) : tm :=
+  match n with
+  | O => tempty
+  | S n' => tpair tempty (rc_create n')
+  end.
+
+Fixpoint rc_length (rc : tm) : nat :=
+  match rc with
+  | tpair _ rc' => S (rc_length rc')
+  | _ => O
+  end.
+
+Fixpoint rc_read (n : nat) (rc : tm) : tm :=
+  match n with
+  | O =>
+    match rc with
+    | tpair t1 _ => t1
+    | _ => tempty
+    end
+  | S n' =>
+    match rc with
+    | tpair _ rc' => rc_read n' rc'
+    | _ => tempty
+    end
+  end.
+
+Fixpoint rc_write (n : nat) (t rc : tm) : tm :=
+  match n with
+  | O =>
+    match rc with
+    | tpair _ rc' => tpair t rc'
+    | _ => rc
+    end
+  | S n' =>
+    match rc with
+    | tpair t1 rc' => tpair t1 (rc_write n' t rc')
+    | _ => rc
+    end
+  end.
+
+Lemma rc_create_is_rc:
+  forall n,
+  is_rc (rc_create n).
+Proof with auto.
+  induction n; simpl; constructor...
+  Qed.
+
+Lemma rc_create_length:
+  forall n,
+  rc_length (rc_create n) = n.
+Proof with auto.
+  induction n; simpl...
+  Qed.
+
+Lemma rc_create_correct:
+  forall n m,
+  lt m n ->
+  rc_read m (rc_create n) = tempty.
+Proof with auto.
+  induction n. intros. inversion H.
+  destruct m; simpl...
+  Qed.
+
+Lemma rc_read_overflow:
+  forall rc,
+  is_rc rc ->
+  forall m,
+    le (rc_length rc) m ->
+    rc_read m rc = tempty.
+Proof with auto.
+  intros rc H. induction H; destruct m...
+  simpl. intros. inversion H0.
+  simpl. intros. apply Le.le_S_n in H0...
+  Qed.
+
+Lemma rc_write_is_rc:
+  forall rc,
+  is_rc rc ->
+  forall n t,
+    is_rc (rc_write n t rc).
+Proof with auto.
+  intros rc H.
+  induction H; destruct n; simpl; constructor...
+  Qed.
+
+Lemma rc_write_length:
+  forall rc,
+  is_rc rc ->
+  forall n t,
+    rc_length (rc_write n t rc) = rc_length rc.
+Proof with auto.
+  intros rc H. induction H.
+  destruct n; simpl; constructor...
+  destruct n; simpl...
+  Qed.
+
+Lemma rc_write_correct_1:
+  forall rc,
+  is_rc rc ->
+  forall n m t,
+    lt m (rc_length rc) ->
+    m <> n ->
+    rc_read m (rc_write n t rc) = rc_read m rc.
+Proof with auto.
+  intros rc H. induction H.
+  simpl. intros. inversion H.
+  destruct n.
+  destruct m... intros. exfalso...
+  destruct m...
+  simpl. intros. apply not_eq_n in H1...
+  Qed.
+
+Lemma rc_write_correct_2:
+  forall rc,
+  is_rc rc ->
+  forall n t,
+    lt n (rc_length rc) ->
+    rc_read n (rc_write n t rc) = t.
+Proof with auto.
+  intros rc H. induction H.
+  intros. inversion H.
+  destruct n...
+  simpl. intros...
+  Qed.
+
+End Records.
 
 Reserved Notation "t1 '/' st1 '==>' t2 '/' st2"
   (at level 40, st1 at level 39, t2 at level 39).
